compcert_new/cfrontend/Clight.v
@@ -780,9 +780,7 @@ Inductive entry_point (ge:genv): mem -> state -> val -> list val -> Prop :=
                            && zlt (4*(2*(Zlength args))) Int.max_unsigned = true ->*)
       Genv.find_funct_ptr ge b0 = Some (Internal f0) ->
       Mem.alloc m0 0 0 = (m1, stk) ->
-      entry_point ge m0 (Callstate f args (Kcall None f0 empty_env
-                                                 (temp_bindings
-                                                    1%positive (Vptr fb Ptrofs.zero::args)) Kstop) m1) (Vptr fb Ptrofs.zero) args.
+      entry_point ge m0 (Callstate f args Kstop m1) (Vptr fb Ptrofs.zero) args.
 
 (** A final state is a [Returnstate] with an empty continuation. *)
 Inductive final_state: state -> int -> Prop :=
