concurrency/juicy/semax_invariant.v
@@ -284,7 +284,7 @@ Definition threads_safety m (tp : jstate ge) PHI (mcompat : mem_compatible_with 
     | Kinit v1 v2 =>
       val_inject (Mem.flat_inj (Mem.nextblock m)) v2 v2 /\
       exists q_new,
-      veric.Clight_core.cl_initial_core ge v1 (v2 :: nil) = Some q_new /\
+      veric.Clight_core.cl_initial_core ge v1 (v2 :: nil) q_new /\
       jsafe_phi ge n ora q_new (getThreadR cnti)
     end.
 
